Sudoku/Lemmas.lean
@@ -70,6 +70,95 @@ lemma col_elim {g : Grid} (hg : SudokuRules g) {col a : Fin 4} {n : ℕ} (hn : n
     exact hn
   · exact h_col a' ha'
 
+lemma reg_coords_rw (c : Coords) : c = reg_coords (c.1 / 2 * 2 + c.2 / 2) (c.1 % 2 * 2 + c.2 % 2) := by
+  unfold reg_coords
+  have h : 4 = 2 * 2 := by norm_num
+  conv =>
+    right
+    congr
+    · rw [Fin.add_def]
+      left
+      rw [Fin.val_mul, Fin.div_val, Fin.val_add, Fin.val_mul]
+      simp
+      simp only [h]
+      rw [Nat.mod_mul_right_div_self, Nat.add_div_of_dvd_right (by simp), @Nat.div_eq_of_lt (c.2 / 2) 2 (Nat.div_lt_of_lt_mul c.2.isLt)]
+      simp
+      rw [@Nat.mod_eq_of_lt (c.1 / 2) 2 (Nat.div_lt_of_lt_mul c.1.isLt), Fin.val_add, Fin.val_mul]
+      simp
+      simp only [h]
+      rw [Nat.mod_mul_right_div_self, Nat.add_div_of_dvd_right (by simp)]
+      simp
+      rw [Nat.div_add_mod', Nat.mod_eq_of_lt (c.1.isLt)]
+    · rw [Fin.add_def]
+      left
+      rw [Fin.val_mul, Fin.mod_val, Fin.val_add, Fin.val_mul]
+      simp
+      rw [Nat.mod_mod_of_dvd _ (by norm_num), Nat.add_mod _ _ 2, Nat.mul_mod_left]
+      simp
+      rw [@Nat.mod_eq_of_lt (c.2 / 2) 2 (Nat.div_lt_of_lt_mul c.2.isLt), Fin.val_add, Fin.val_mul]
+      simp
+      rw [Nat.mod_mod_of_dvd _ (by norm_num), Nat.add_mod _ _ 2, Nat.mul_mod_left]
+      simp
+      rw [Nat.div_add_mod', Nat.mod_eq_of_lt (c.2.isLt)]
+
 lemma reg_conflict {g : Grid} (hg : SudokuRules g) {c₁ c₂ : Coords} (hc : c₁ ≠ c₂) (hc' : c₁.1 / 2 = c₂.1 / 2 ∧ c₁.2 / 2 = c₂.2 / 2) (hg' : g c₁ = n) : g c₂ ≠ n := by
-  rw [←hg']
-  exact Ne.symm (hg.reg_check _ _ hc hc')
+  rw [←hg', reg_coords_rw c₂, reg_coords_rw c₁, hc'.1, hc'.2]
+  apply hg.reg_check
+  contrapose! hc
+  rw [Prod.eq_iff_fst_eq_snd_eq]
+  conv at hc' =>
+    congr <;> {
+      simp [Fin.ext_iff, Fin.div_val]
+    }
+  have h : 4 = 2 * 2 := by norm_num
+  constructor
+  · apply Fin.eq_of_val_eq
+    rw [←Nat.div_add_mod' c₁.1 2, ←Nat.div_add_mod' c₂.1 2]
+    replace hc := congrArg (fun a => a.val / 2) hc
+    conv at hc =>
+      simp
+      congr <;> {
+        rw [Fin.val_add, Fin.val_mul, Fin.mod_val, Fin.mod_val]
+        simp
+        simp only [h]
+        rw [Nat.mod_mul_right_div_self, Nat.add_div_of_dvd_right (by simp)]
+        simp
+      }
+    rw [hc'.1, hc]
+  · apply Fin.eq_of_val_eq
+    rw [←Nat.div_add_mod' c₁.2 2, ←Nat.div_add_mod' c₂.2 2]
+    replace hc := congrArg (fun a => a.val % 2) hc
+    conv at hc =>
+      simp
+      congr <;> {
+        rw [Fin.val_add, Fin.val_mul, Fin.mod_val, Fin.mod_val]
+        simp
+        rw [Nat.mod_mod_of_dvd _ (by norm_num), Nat.add_mod]
+        simp
+      }
+    rw [hc'.2, hc]
+
+def reg_emb {g : Grid} (hg : SudokuRules g) (reg : Fin 4) : Fin 4 ↪ ℕ where
+  toFun := fun a => g (reg_coords reg a)
+  inj' := by
+    intro a b hab
+    contrapose! hab
+    exact hg.reg_check reg a b hab
+
+lemma reg_map {g : Grid} (hg : SudokuRules g) (reg : Fin 4) : Finset.map (reg_emb hg reg) Finset.univ = Finset.Icc 1 4 := by
+  apply Finset.eq_of_subset_of_card_le
+  · intro n hn
+    simp [reg_emb] at hn
+    obtain ⟨a, ha⟩ := hn
+    rw [←ha]
+    apply hg.cases
+  · simp
+
+lemma reg_elim {g : Grid} (hg : SudokuRules g) {c : Coords} {n : ℕ} (hn : n ∈ Finset.Icc 1 4) (h_reg : ∀ c' : Fin 4, c' ≠ c.1 % 2 * 2 + c.2 % 2 → g (reg_coords (c.1 / 2 * 2 + c.2 / 2) c') ≠ n) : g c = n := by
+  simp [←reg_map hg (c.1 / 2 * 2 + c.2 / 2), reg_emb] at hn
+  contrapose! hn
+  intro a
+  obtain ha | ha := eq_or_ne a (c.1 % 2 * 2 + c.2 % 2)
+  · rw [ha, ←reg_coords_rw]
+    exact hn
+  · exact h_reg a ha
